Comments and make ground types implicit

QueryLanguage/Basic.lean
@@ -1,47 +1,108 @@
+/-!
+  This is a core setup for a query language thats acts as an interface
+  between Lean and a database. There is no presumption here about how the
+  database is implemented, we only assume that it knows how to execute
+  queries.
 
+  The end user would not use these types directly. There will be another
+  layer that translates user queries.
+
+  Everything below is a scaffolding that needs to be fleshed out.
+  (For example, there is only conjunction, but it should be easy to add more logic.)
+-/
+
+
+/-- The types of terms appearing in a query. It is parameterized by
+    a type of ground types that the database knows about. At present
+    we only support n-tuples, coded as nested pairs, as they are needed to
+    implement n-ary primitive functions and primitive predicates.
+
+    Think of the elements of `Ty Ground` as *codes* of types.
+-/
 inductive Ty (Ground : Type) where
   | unit : Ty Ground
   | ground : Ground → Ty Ground
   | prod : Ty Ground → Ty Ground → Ty Ground
 
+/-- Given an interpretation of ground types, we can interpret
+    any type (code) as a Lean type. -/
 def Ty.interpret {G : Type} (I : G → Type) : Ty G → Type
   | .unit => Unit
   | .ground g => I g
   | .prod t u => t.interpret I × u.interpret I
 
+/-- An operation signature specifies which primitive operations
+    can appear in the terms in queries. Typical examples might be
+    arithmetical operations.
+-/
 structure OpSignature (Ground : Type) where
+  /-- operation sysmbols -/
   op : Type
+  /-- the domain of an operation symbol -/
   dom : op → Ty Ground
+  /-- the codomain of an operation symbol -/
   cod : op → Ty Ground
 
+/-- A predicate signature specifies which primitive predicates
+    (relations) can appear in queries. Typical examples might
+    be arithmetical comparison `<` and equality `=`.
+    Note that each type may be equipped with its own notion of
+    equality, but need not to.
+-/
 structure PredSignature (Ground : Type) where
+  /-- predicate symbols -/
   pred : Type
+  /-- the domain of a predicate symbol -/
   dom : pred → Ty Ground
 
+/-- The capabilities of a database are described by a signature.
+    At present we just assume that each entry (mathematical object)
+    in the database has some attributes (e.g. columns or views).
+
+    Queries to the database can refer to the attributes as if they
+    were 0-ary operations.
+ -/
 structure DBSignature (G : Type) where
+  /-- the attributes -/
   attr : Type
+  /-- the type of an attribute -/
   ty : attr → Ty G
 
-inductive Tm (G : Type) (O : OpSignature G) (D : DBSignature G): Ty G → Type where
-| tt : Tm G O D Ty.unit
-| pair : ∀ {A B : Ty G}, Tm G O D A → Tm G O D B → Tm G O D (.prod A B)
-| fst : ∀ {A B : Ty G}, Tm G O D (.prod A B) → Tm G O D A
-| snd : ∀ {A B : Ty G}, Tm G O D (.prod A B) → Tm G O D B
-| app : ∀ (f : O.op), Tm G O D (O.dom f) → Tm G O D (O.cod f)
-| get : ∀ (c : D.attr), Tm G O D (D.ty c)
+/-- The terms that may appear in a query. -/
+inductive Tm {G : Type} (O : OpSignature G) (D : DBSignature G): Ty G → Type where
+| tt : Tm O D Ty.unit
+| pair : ∀ {A B : Ty G}, Tm O D A → Tm O D B → Tm O D (.prod A B)
+| fst : ∀ {A B : Ty G}, Tm O D (.prod A B) → Tm O D A
+| snd : ∀ {A B : Ty G}, Tm O D (.prod A B) → Tm O D B
+| app : ∀ (f : O.op), Tm O D (O.dom f) → Tm O D (O.cod f)
+| get : ∀ (c : D.attr), Tm O D (D.ty c)
 
-inductive Query (G : Type) (O : OpSignature G) (P : PredSignature G) (D : DBSignature G) where
-| fal : Query G O P D
-| tru : Query G O P D
-| conj : Query G O P D → Query G O P D → Query G O P D
-| pred : ∀ (p : P.pred), Tm G O D (P.dom p) → Query G O P D
 
-structure DB (G : Type) (I : G → Type) (O : OpSignature G) (P : PredSignature G) (D : DBSignature G) where
+/-- A query is a logical formula. -/
+inductive Query {G : Type} (O : OpSignature G) (P : PredSignature G) (D : DBSignature G) where
+| fal : Query O P D
+| tru : Query O P D
+| conj : Query O P D → Query O P D → Query O P D
+| pred : ∀ (p : P.pred), Tm O D (P.dom p) → Query O P D
+
+/-- A database stores objects of a given type `Obj`. It specifies how
+    the attributes are interpreted, and it can execute queries that fetch
+    lists of objects. In the future we will likely replace lists with
+    a more suitable datastructure, such as a stream or an iterator. -/
+structure DB {G : Type} (I : G → Type) (O : OpSignature G) (P : PredSignature G) (D : DBSignature G) where
+  /-- The type of objects stored in the database -/
   Obj : Type
+  /-- For a given object and an attribute, return its value -/
   get : Obj → ∀ (a : D.attr), (D.ty a).interpret I
-  exec : Query G O P D → List Obj
+  /-- Execute a query and return the list of objects satisfying it -/
+  exec : Query O P D → List Obj
 
 namespace Peano
+  /-! An example of a query language that supports natural numbers,
+    numeral constants, addition, equality =, the "even" predicate,
+    and the attributes `size` and `genus` (this is made up).
+  -/
+
   inductive Ground where
   | nat : Ground
 
@@ -86,6 +147,7 @@ namespace Peano
   | size : Attr
   | genus : Attr
 
+  /-- `size` returns natural numbers and `genus` returns pairs of natural numbers -/
   @[reducible]
   def Attr.ty : Attr → Ty Ground
   | .size => .ground .nat
@@ -99,14 +161,21 @@ namespace Peano
 end Peano
 
 namespace MyDB
+  /-! A small database, implemented simply as a list of
+      objects. -/
+
   open Peano
 
+  /-- The database stores a bunch of cows, where each cow
+      is given by a list of numbers and a genus. -/
   structure Cow where
     elems : List Nat
     genus : Nat × Nat
 
+  /-- The size of a cow is the length of its list. -/
   def Cow.size (c : Cow) : Nat := c.elems.length
 
+  /-- The information stored in the database. -/
   def pasture : List Cow := [
     { elems := [1,2,3,4],
       genus := (2, 3)},
@@ -122,30 +191,35 @@ namespace MyDB
       genus := (1, 0)},
   ]
 
-  def CowDB : DB Ground Ground.interpret opSignature predSignature dbSignature where
+  /-- The database -/
+  def CowDB : DB Ground.interpret opSignature predSignature dbSignature where
     Obj := Cow
     get := (fun (c : Cow) (a : Attr) => match a with
               | .size => c.size
               | .genus => c.genus
            )
-    exec := (fun (q : Query _ _ _ _) => pasture.filter (fun _ => True) )
+    /- TODO implement this -/
+    exec := (fun (q : Query _ _ _) => pasture.filter (fun _ => True) )
 
 end MyDB
 
 section Example
+  /-! Usage examples. Note that writing queries by hand is quite
+      annoying at present, but we shall improve this bit. -/
+
   open Peano
 
   def ten :=
-    (.app (Op.const 10) .tt : Tm Ground opSignature dbSignature _)
+    (.app (Op.const 10) .tt : Tm opSignature dbSignature _)
 
   def get_size :=
-    (.get Attr.size : Tm Ground opSignature dbSignature _)
+    (.get Attr.size : Tm opSignature dbSignature _)
 
   def get_genus :=
-    (.get Attr.genus : Tm Ground opSignature dbSignature _)
+    (.get Attr.genus : Tm opSignature dbSignature _)
 
-  -- objects of size 10 whose first component of genus is even
-  example: Query Ground opSignature predSignature dbSignature :=
+  -- query: objects of size 10 whose first component of genus is even
+  example: Query opSignature predSignature dbSignature :=
     .conj
       (.pred .eq (.pair get_size ten))
       (.pred .even (.fst get_genus))
